
# Basis to Matrix and Change of Basis

## 1. What Is a Basis?

A **basis** of a vector space is a set of vectors that:

1. Are **linearly independent**
2. **Span the space**

Given a basis, **every vector** in the space can be written as a **linear combination** of the basis vectors.

The **scalars** used in this linear combination are called the **coordinates of the vector with respect to that basis**.

---

## 2. Standard Basis in 2D

The **standard basis** for $\mathbb{R}^2$ is:


[
$\mathcal{B}_\text{std} = 
$
{
$
\begin{bmatrix}
1 \\
0
\end{bmatrix},
$
$
\begin{bmatrix}
0 \\
1
\end{bmatrix}
$}
]

These vectors lie along:

* X-axis
* Y-axis

They are:

* Linearly independent
* Span the 2D plane

---

## 3. Vector Representation Using Standard Basis

Consider the vector:
$[
\mathbf{v} =
\begin{bmatrix}
2 \\
3
\end{bmatrix}
]$

Using the standard basis:

$[
\mathbf{v}
= 2
$
$
\begin{bmatrix}
1 \\
0
\end{bmatrix}
$ * 3
 $
\begin{bmatrix}
  0 \\
  1
  \end{bmatrix}
$
]

So the **coordinates** of $\mathbf{v}$ in the standard basis are:
$[
(2,,3)
]$

---

## 4. Matrix Representation of a Basis

A basis can be written as a **matrix whose columns are the basis vectors**.

For the standard basis:
$[
B_1 =
\begin{bmatrix}
1 & 0 \\
0 & 1
\end{bmatrix}
]$

Then:
$[
\mathbf{v} = B_1
\begin{bmatrix}
2 \\
3
\end{bmatrix}
]$

---

## 5. Same Vector, Different Basis

Now consider a **different basis**:
$[
\mathcal{B}_2 =
\{
\begin{bmatrix}
1 \\
1
\end{bmatrix},
\begin{bmatrix}
0 \\
1
\end{bmatrix}
\}
]$

The **same vector** $\mathbf{v} = (2,3)$ can also be written as:

$[
\mathbf{v}
= (-1)
\begin{bmatrix}
1 \\
1
\end{bmatrix} * 3
  \begin{bmatrix}
  0 \\
  1
  \end{bmatrix}
]$

So its **coordinates in basis $\mathcal{B}_2$** are:
$[
(-1,,3)
]$

ðŸ‘‰ **Vector is the same, coordinates change**

---

## 6. Basis Matrix for the New Basis

Write the basis vectors as columns:
$[
B_2 =
\begin{bmatrix}
1 & 0 \\
1 & 1
\end{bmatrix}
]$

Then:
$[
\mathbf{v} = B_2
\begin{bmatrix}
-1 \\
3
\end{bmatrix}
]$

---

## 7. Key Idea: Coordinates Depend on the Basis

* A vector itself does **not** change
* Its **coordinates depend on the basis**
* Changing the basis changes the numbers used to represent the same vector

---

# Change of Basis

## 8. General Change of Basis Formula

Let:

* $B_1$ = old basis matrix
* $B_2$ = new basis matrix
* $[\mathbf{v}]_{B_1}$ = coordinates in basis $B_1$
* $[\mathbf{v}]_{B_2}$ = coordinates in basis $B_2$

Since the vector is the same:
$[
B_1[\mathbf{v}]*{B_1} = B_2[\mathbf{v}]*{B_2}
]$

Solving for new coordinates:
$[
[\mathbf{v}]*{B_2} = B_2^{-1} B_1 [\mathbf{v}]*{B_1}
]$

---

## 9. Example: Standard Basis to New Basis

### Given

$[
[\mathbf{v}]_{B_1} =
\begin{bmatrix}
2 \\
3
\end{bmatrix},
\quad
B_1 = I
]$

$[
B_2 =
\begin{bmatrix}
1 & 0 \\
1 & 1
\end{bmatrix}
]$

---

### Step 1: Compute $B_2^{-1}$

Determinant:
$[
\det(B_2) = 1 \cdot 1 - 0 \cdot 1 = 1
]$

$[
B_2^{-1} =
\begin{bmatrix}
1 & 0 \\
-1 & 1
\end{bmatrix}
]$

---

### Step 2: Compute New Coordinates

$[
[\mathbf{v}]_{B_2} = B_2^{-1}
\begin{bmatrix}
2 \\
3
\end{bmatrix}
=
\begin{bmatrix}
2 \\
1
\end{bmatrix}
]$

âœ”ï¸ Coordinates of $\mathbf{v}$ in basis $B_2$

---

## 10. Another Example

Let:
$[
B_2 =
\begin{bmatrix}
2 & 1 \\
1 & 2
\end{bmatrix},
\quad
\mathbf{v} =
\begin{bmatrix}
2 \\
3
\end{bmatrix}
]$

### Inverse of $B_2$:

$[
\det(B_2) = 4 - 1 = 3
]$

$[
B_2^{-1} =
\frac{1}{3}
\begin{bmatrix}
2 & -1 \\
-1 & 2
\end{bmatrix}
]$

### New coordinates:

$[
[\mathbf{v}]_{B_2}
=
\frac{1}{3}
\begin{bmatrix}
2 & -1 \\
-1 & 2
\end{bmatrix}
\begin{bmatrix}
2 \\
3
\end{bmatrix}
=
\begin{bmatrix}
\frac{1}{3} \
\frac{4}{3}
\end{bmatrix}
]$

---

## 11. Final Rule (Very Important)

> **To find coordinates of a vector in a given basis:**

$[
\boxed{
[\mathbf{v}]_{\text{basis}}
=
(\text{basis matrix})^{-1}
\mathbf{v}
}
]$

---

## 12. Key Takeaways

* Basis vectors define the coordinate system
* A vector is **independent of basis**
* Coordinates depend on the basis
* Change of basis uses **matrix inverse**
* This idea is crucial for:

  * Eigenvectors
  * PCA
  * Diagonalization
  * ML feature spaces

--------------------


# Change of Basis (Part 2)

## 1. Concept: Vector in Different Bases

Suppose we have:

* A vector $\mathbf{U}$
* Two bases:
  $[
  B_1 = {\mathbf{b}_1, \mathbf{b}_2}, \quad B_2 = {\mathbf{b}_1', \mathbf{b}_2'}
  ]$

Let:
[
$[\mathbf{U}]*{B_1} = \text{coordinates of } \mathbf{U} \text{ in basis } B_1$
]
[
$[\mathbf{U}]*{B_2} = \text{coordinates of } \mathbf{U} \text{ in basis } B_2$
]

We want to **compute the coordinates of $\mathbf{U}$ in $B_2$** when we know its coordinates in $B_1$.

---

## 2. Represent the Vector in Both Bases

Vector in $B_1$:
[
$\mathbf{U} = B_1 [\mathbf{U}]_{B_1}$
]

Vector in $B_2$:
[
$\mathbf{U} = B_2 [\mathbf{U}]_{B_2}$
]

Since it is the **same vector**:
[
$B_1 [\mathbf{U}]*{B_1} = B_2 [\mathbf{U}]*{B_2}$
]

---

## 3. Solve for New Coordinates

Multiply both sides by $B_2^{-1}$:
[
$[\mathbf{U}]*{B_2} = B_2^{-1} B_1 [\mathbf{U}]*{B_1}$
]

âœ… This is the **matrix formula for change of basis**.

---

## 4. Example

### Given

* Vector coordinates in $B_1$:
  $[
  [\mathbf{U}]_{B_1} =
  \begin{bmatrix}
  2 \\
  2
  \end{bmatrix}
  ]$

* Basis matrices:
  $[
  B_1 =
  \begin{bmatrix}
  1 & 0 \\
  0 & 1
  \end{bmatrix}, \quad
  B_2 =
  \begin{bmatrix}
  1 & 1 \\
  0 & 1
  \end{bmatrix}
  ]$

---

### Step 1: Compute $B_2^{-1}$

$[
\det(B_2) = 1 \cdot 1 - 1 \cdot 0 = 1
]$

$[
B_2^{-1} =
\begin{bmatrix}
1 & -1 \\
0 & 1
\end{bmatrix}
]$

---

### Step 2: Compute New Coordinates

$[
[\mathbf{U}]*{B_2} = B_2^{-1} B_1 [\mathbf{U}]*{B_1}
=
\begin{bmatrix}
1 & -1 \\
0 & 1
\end{bmatrix}
\begin{bmatrix}
1 & 0 \\
0 & 1
\end{bmatrix}
\begin{bmatrix}
2 \\
2
\end{bmatrix}
=
\begin{bmatrix}
0 \\
2
\end{bmatrix}
]$

---

### Step 3: Visual Interpretation

* Same vector $\mathbf{U}$ is plotted in **two different coordinate systems**
* In $B_1$ coordinates: $(2,2)$
* In $B_2$ coordinates: $(0,2)$
* Vector direction and length **unchanged**, but **coordinates relative to axes changed**

---

## 5. Summary: Change of Basis Formula

$[
\boxed{
[\mathbf{U}]*\text{new} = B*\text{new}^{-1} B_\text{old} [\mathbf{U}]_\text{old}
}
]$

* $B_\text{old}$ = matrix of old basis vectors
* $B_\text{new}$ = matrix of new basis vectors
* $[\mathbf{U}]_\text{old}$ = coordinates in old basis
* $[\mathbf{U}]_\text{new}$ = coordinates in new basis

> âœ… Key point: The **vector itself does not change**, only the **coordinates** do.

----

# Change of Basis Matrix

## 1. Concept

Suppose we have:

* Two bases: $B_1$ and $B_2$
* Coordinates of a vector $\mathbf{U}$ in **basis $B_1$**: $[\mathbf{U}]_{B_1}$
* We want coordinates of the same vector in **basis $B_2$**: $[\mathbf{U}]_{B_2}$

---

## 2. Change of Basis Matrix

The **change of basis matrix** $C$ from $B_2$ to $B_1$ is defined as:

$[
C = B_2^{-1} B_1
]$

* $B_1$ = matrix of old basis vectors (columns)
* $B_2$ = matrix of new basis vectors (columns)
* $C$ converts coordinates in $B_1$ to coordinates in $B_2$:

[
$[\mathbf{U}]*{B_2} = C , [\mathbf{U}]*{B_1}$
]

---

## 3. Inverse Change of Basis

Similarly, if we already have coordinates in $B_2$ and want them in $B_1$, we use the **inverse of the change of basis matrix**:

[
$[\mathbf{U}]*{B_1} = C^{-1} , [\mathbf{U}]*{B_2}$
]

* Visually: Multiply by $C$ to go **from old basis â†’ new basis**
* Multiply by $C^{-1}$ to go **from new basis â†’ old basis**

---

## 4. Step-by-Step Procedure

Given:

* Bases $B_1$ and $B_2$
* Coordinates $[\mathbf{U}]_{B_1}$

To find $[\mathbf{U}]_{B_2}$:

1. Construct basis matrices:
   $[
   B_1 = [\mathbf{b}_1 \ \mathbf{b}_2], \quad
   B_2 = [\mathbf{b}_1' \ \mathbf{b}_2']
   ]$

2. Compute the **inverse** of $B_2$:
   $[
   B_2^{-1}
   ]$

3. Compute the **change of basis matrix**:
   $[
   C = B_2^{-1} B_1
   ]$

4. Multiply coordinates in $B_1$ by $C$ to get coordinates in $B_2$:
   $[
   [\mathbf{U}]*{B_2} = C , [\mathbf{U}]*{B_1}
   ]$

---

## 5. Example

Suppose:

$[
B_1 =
\begin{bmatrix}
1 & 0 \\
0 & 1
\end{bmatrix}, \quad
B_2 =
\begin{bmatrix}
1 & 1 \\
0 & 1
\end{bmatrix}, \quad
[\mathbf{U}]_{B_1} =
\begin{bmatrix}
2 \\
2
\end{bmatrix}
]$

**Step 1: Compute $B_2^{-1}$**

$[
\det(B_2) = 1 \cdot 1 - 1 \cdot 0 = 1
]$

$[
B_2^{-1} =
\begin{bmatrix}
1 & -1 \\
0 & 1
\end{bmatrix}
]$

**Step 2: Compute change of basis matrix**

$[
C = B_2^{-1} B_1 =
\begin{bmatrix}
1 & -1 \\
0 & 1
\end{bmatrix}
\begin{bmatrix}
1 & 0 \\
0 & 1
\end{bmatrix}
=
\begin{bmatrix}
1 & -1 \\
0 & 1
\end{bmatrix}
]$

**Step 3: Compute coordinates in $B_2$**

$[
[\mathbf{U}]*{B_2} = C , [\mathbf{U}]*{B_1}
=
\begin{bmatrix}
1 & -1 \\
0 & 1
\end{bmatrix}
\begin{bmatrix}
2 \\
2
\end{bmatrix}
=
\begin{bmatrix}
0 \\
2
\end{bmatrix}
]$

âœ… Same vector, new coordinates.

---

### 6. Summary

$$
\begin{aligned}
C &= B_2^{-1} B_1 \quad \text{(change of basis matrix from } B_1 \to B_2\text{)} \\
[\mathbf{U}]_{B_2} &= C \,[\mathbf{U}]_{B_1} \\
[\mathbf{U}]_{B_1} &= C^{-1} \,[\mathbf{U}]_{B_2}
\end{aligned}
$$



> The **change of basis matrix** is the key tool for transforming vector coordinates between any two bases.


---

## Transformation in a Different Basis

Previously, all transformations were performed in the **standard basis**
$[
B_1 = {(1,0),(0,1)}.
]$
In that basis, standard transformations such as reflection, rotation, dilation, and shear are represented by well-known matrices.

However, **if a vector is given in a different basis**, say (B_2), **we cannot directly use those same matrices**.
Instead, we must convert the vector to the standard basis, apply the transformation, and then convert it back.

---

## Standard Transformations in the Standard Basis

For example, reflection about the (x)-axis in the standard basis is given by:
$[
T =
\begin{bmatrix}
1 & 0 \\
0 & -1
\end{bmatrix}
]$

This matrix **only works in the standard basis**.

---

## Why the Same Matrix Cannot Be Used in Another Basis

If a vector $([\mathbf{u}]_{B_2}) is expressed in a non-standard basis (B_2), the matrix (T) above does **not** correctly reflect the vector in that basis.$

So we need a **new matrix** that represents the same transformation **with respect to the basis (B_2)**.

---

## Change of Basis Idea

Let:

* $(C = B_2^{-1} B_1) be the **change-of-basis matrix** (from (B_2) to (B_1))$
* $(T) be the transformation matrix in the **standard basis**$

---

## Steps to Transform a Vector in a Different Basis

$Suppose we have a vector ([\mathbf{u}]_{B_2}) and want to apply transformation (T) **in the same basis (B_2)**.$

### Step 1: Convert to standard basis

$[
[\mathbf{u}]*{B_1} = C ,[\mathbf{u}]*{B_2}
]$

### Step 2: Apply the transformation

$[
[\mathbf{v}]*{B_1} = T ,[\mathbf{u}]*{B_1}
]$

### Step 3: Convert back to the original basis

$[
[\mathbf{v}]*{B_2} = C^{-1} ,[\mathbf{v}]*{B_1}
]$

---

## Final Transformation Formula (Most Important)

Combining all steps:
$[
[\mathbf{v}]_{B_2}
=
C^{-1} , T , C ,[\mathbf{u}]_{B_2}
]$

âœ… This matrix
$[
T_{B_2} = C^{-1} T C
]$
is the **representation of the transformation in basis $(B_2)$**.

---

## Key Takeaway

* **Transformation matrices depend on the basis**
* To apply a standard transformation in a different basis:

  1. Convert to standard basis
  2. Apply the transformation
  3. Convert back

This idea is central to **linear transformations, diagonalization, and similarity of matrices**.


---

## Transformation in a Different Basis â€“ 2

Suppose you want to **reflect a vector whose coordinates are**
$[
[\mathbf{u}]_{B_2}
]$
in the basis
$[
B_2.
]$

Since reflection matrices are defined with respect to the **standard basis**, we **cannot apply them directly** in a non-standard basis. Instead, we follow a three-step process.

---

## Step 1: Convert the vector to the standard basis

If the basis matrix corresponding to (B_2) is
$[
B_2 = \begin{bmatrix}
\mathbf{b}_1 & \mathbf{b}*2
\end{bmatrix},
]$
then the actual vector in the standard basis is:
$[
\mathbf{u} = B_2 ,[\mathbf{u}]*{B_2}
]$

---

## Step 2: Apply reflection in the standard basis

Reflection about the **x-axis** in the standard basis is given by:
$[
T =
\begin{bmatrix}
1 & 0 \\
0 & -1
\end{bmatrix}
]$

Applying the transformation:
$[
\mathbf{v} = T \mathbf{u}
]$

This gives the **reflected vector in the standard basis**.

---

## Step 3: Convert the reflected vector back to basis (B_2)

To get the coordinates in the original basis:
$[
[\mathbf{v}]_{B_2} = B_2^{-1} \mathbf{v}
]$

---

## Combined Transformation Formula

Substituting all steps into a single expression:
$[
[\mathbf{v}]_{B_2}
=
B_2^{-1} , T , B_2 ,[\mathbf{u}]_{B_2}
]$

This matrix
$[
T_{B_2} = B_2^{-1} T B_2
]$
is the **reflection matrix in basis (B_2)**.

---

## Worked Example

### Given:

* Vector in basis (B_2):
  $[
  [\mathbf{u}]_{B_2} =
  \begin{bmatrix}
  1 \\
  1
  \end{bmatrix}
  ]$

* Basis vectors:
  $[
  B_2 =
  \{
  \begin{bmatrix} 2 \\ 1 \end{bmatrix},
  \begin{bmatrix} 1 \\ 2 \end{bmatrix}
  \}
  ]$

So the basis matrix is:
$[
B_2 =
\begin{bmatrix}
2 & 1 \\
1 & 2
\end{bmatrix}
]$

---

### Step 1: Convert to standard basis

$[
\mathbf{u} = B_2
\begin{bmatrix}
1 \\
1
\end{bmatrix}
=
\begin{bmatrix}
3 \\
3
\end{bmatrix}
]$

---

### Step 2: Reflect in standard basis

$[
\mathbf{v} =
\begin{bmatrix}
1 & 0 \\
0 & -1
\end{bmatrix}
\begin{bmatrix}
3 \\
3
\end{bmatrix}
=
\begin{bmatrix}
3 \\
-3
\end{bmatrix}
]$

---

### Step 3: Convert back to basis (B_2)

First compute:
$[
B_2^{-1}
=
\frac{1}{3}
\begin{bmatrix}
2 & -1 \\
-1 & 2
\end{bmatrix}
]$

Now:
$[
[\mathbf{v}]_{B_2}
=
\frac{1}{3}
\begin{bmatrix}
2 & -1 \\
-1 & 2
\end{bmatrix}
\begin{bmatrix}
3 \\
-3
\end{bmatrix}
=
\begin{bmatrix}
3 \\
3
\end{bmatrix}
]$

---

## Final Answer

$[
\boxed{
[\mathbf{v}]_{B_2} =
\begin{bmatrix}
3 \\
3
\end{bmatrix}
}
]$

---

## Key Takeaway

To perform **any linear transformation in a non-standard basis**:

1. Convert the vector to the standard basis
2. Apply the transformation
3. Convert the result back to the original basis

Mathematically:
$[
[\mathbf{v}]_{B}
=
B^{-1} T B ,[\mathbf{u}]_{B}
]$

---
